algebras 2

Cslib/Foundations/Semantics/Algebra/Basic.lean
@@ -143,4 +143,90 @@ instance instPiSAlgebra {κ : Type _} (As : κ → Type _) [∀ k, SAlgebra S (A
     SAlgebra S (Π k, As k) where
   interp f xs k := interp f (fun i => xs i k)
 
+open Term PTree
+
+variable {X : Type u}
+
+instance instSAlgebraTerm (S : Signature) (X : Type u) : SAlgebra S (Term S X) where
+  interp f xs := consNodeOfFn f xs
+
+def liftTermAlgebra {A : Type u} [SAlgebra S A] (φ : X → A) (t : Term S X) : A :=
+  match t with
+  | ⟨leaf x, _⟩ => φ x
+  | ⟨node f ts, h⟩ => interp f (fun i => liftTermAlgebra φ h.childTerms[i])
+  termination_by t.t.size
+  decreasing_by simpa only [WF.childTerms_get_coe] using size_getElem_lt_size ..
+
+def liftTermAlgebraHom {A : Type u} [SAlgebra S A] (φ : X → A) : Term S X →[S] A where
+  toFun := liftTermAlgebra φ
+  map_interp' xs := by
+    simp only [interp, consNodeOfFn_eq, liftTermAlgebra]
+    congr; ext i; congr; ext
+    rw [WF.childTerms_get_coe]
+    simp
+
+def Models (E : Term S X → Term S X → Prop) (A : Type u) [SAlgebra S A] : Prop :=
+  ∀ (φ : Term S X →[S] A) (s t : Term S X), E s t → φ s = φ t
+
+def IdentifiedIn (s t : Term S X) (A : Type u) [SAlgebra S A] : Prop :=
+  ∀ (φ : Term S X →[S] A), φ s = φ t
+
+notation A " ⊨ " E => Models E A
+notation A " ⊨ " s " ≡ " t => IdentifiedIn s t A
+
+def SemanticConsequence (E : Term S X → Term S X → Prop) (s t : Term S X) : Prop :=
+  ∀ (A : Type u) [SAlgebra S A], (A ⊨ E) → (A ⊨ s ≡ t)
+
+-- open SemanticConsequence
+
+notation s " ≡[" E "] " t => SemanticConsequence E s t
+
+lemma Models.semanticConsequence (E : Term S X → Term S X → Prop) (A : Type u)
+    [SAlgebra S A] (hA : A ⊨ E) : A ⊨ (· ≡[E] ·) := fun φ _ _ hst => hst A hA φ
+
+lemma Models.eq_of_semanticConsequence {E : Term S X → Term S X → Prop} {A : Type u} [SAlgebra S A]
+    (hA : A ⊨ E) {s t : Term S X} (hst : s ≡[E] t) (φ : Term S X →[S] A) : φ s = φ t :=
+  hst A hA φ
+
+theorem SemanticConsequence.fully_invariant (E : Term S X → Term S X → Prop) (s t : Term S X)
+    (h : s ≡[E] t) (φ : Term S X →[S] Term S X) : (φ s) ≡[E] (φ t) :=
+  fun _ _ hA ψ => hA.semanticConsequence E _ (ψ.comp φ) s t h
+
+theorem SemanticConsequence.equivalence (E : Term S X → Term S X → Prop) :
+    Equivalence (· ≡[E] ·) where
+  refl _ _ _ _ _ := rfl
+  symm hst _ _ hA φ := (hA.eq_of_semanticConsequence hst φ).symm
+  trans hst htu _ _ hA φ :=
+    (hA.eq_of_semanticConsequence hst φ).trans (hA.eq_of_semanticConsequence htu φ)
+
+def SemanticConsequence.congruence (E : Term S X → Term S X → Prop) : Congruence S (Term S X) where
+  toRel := SemanticConsequence E
+  iseqv := SemanticConsequence.equivalence E
+  map_interp h A _ hA φ := by
+    simp_rw [φ.map_interp]
+    congr 1; ext i
+    exact hA.eq_of_semanticConsequence (h i) φ
+
+def RewriteEquiv.congruence (E : PTree S.Sym X → PTree S.Sym X → Prop) :
+    Congruence S (Term S X) where
+  toRel := Function.onFun (RewriteEquiv E) Term.t
+  iseqv := Equivalence.comap RewriteEquiv.equivalence t
+  map_interp := by
+    intro f xs ys h
+    simp only [Function.onFun, interp, consNodeOfFn_eq]
+    exact RewriteEquiv.nodeClosed (E := E) |>.apply_ofFn f (t ∘ xs) (t ∘ ys) h
+
+private noncomputable def outHom (E : PTree S.Sym X → PTree S.Sym X → Prop)
+    (φ : Term S X →[S] Quotient (RewriteEquiv.congruence E).Setoid) : Term S X →[S] Term S X :=
+  liftTermAlgebraHom (fun x => (φ <| ⟨leaf x, .leaf_wf⟩).out)
+
+-- private lemma outHom_comp_mk (E : PTree S.Sym X → PTree S.Sym X → Prop)
+--     (φ : Term S X →[S] Quotient (RewriteEquiv.congruence E).Setoid) :
+--       Quotient.mk (RewriteEquiv.congruence E).Setoid ∘ (outHom E φ) = φ := by
+
+/-- `→` direction amounts to showing the conditions of `RewriteEquiv.minimal`, and `←` to showing
+that `RewriteEquiv E` is a `Congruence`, and that `Term S X ⧸ RewriteEquiv E ⊨ E`. -/
+proof_wanted BirkoffTheorem (E : PTree S.Sym X → PTree S.Sym X → Prop) (s t : Term S X) :
+  RewriteEquiv E s t ↔ s ≡[Function.onFun E Term.t] t
+
 end Cslib.SAlgebra
